proofs/itrees/it_lang.v
@@ -59,12 +59,206 @@ From ITree Require Import Rutt RuttFacts.
 
 From ITree Require Import EqAxiom.
 
-From Jasmin Require Import expr it_lib.
+From Jasmin Require Import expr it_lib psem_defs psem.
 
 Import Monads.
 Import MonadNotation.
 Local Open Scope monad_scope.
 
 Obligation Tactic := done || idtac.
+
+(**** ERROR SEMANTICS *******************************************)
+Section Errors.
+
+(* type of errors (this might becom richer) *)
+Variant ErrType : Type := Err : ErrType. 
+(* error events *)
+Definition ErrState : Type -> Type := exceptE ErrType.
+
+(* failT (itree E) R = itree E (option R) *)
+Definition handle_Err {E} : ErrState ~> failT (itree E) :=
+  fun _ _ => Ret (None).
+
+(* Err handler *)
+Definition ext_handle_Err {E: Type -> Type} :
+  ErrState +' E ~> failT (itree E) :=
+  fun _ e =>
+  match e with
+  | inl1 e' => handle_Err _ e'
+  | inr1 e' => Vis e' (pure (fun x => Some x)) end.                        
+(* ErrState interpreter *)
+Definition interp_Err {E: Type -> Type} {A}  
+  (t: itree (ErrState +' E) A) : failT (itree E) A :=
+  interp_fail ext_handle_Err t.
+
+
+(*** auxiliary functions *)
+
+Definition err_get {E: Type -> Type} 
+  `{ErrState -< E} {S} {V} (f: S -> option V) :
+  stateT S (itree E) V :=
+  fun st => match (f st) with
+            | Some v => Ret (st, v)
+            | None => throw Err end.                
+
+Definition err_put {E: Type -> Type} 
+  `{ErrState -< E} {S} (f: S -> option S) :
+  stateT S (itree E) unit :=
+  fun st => match (f st) with
+            | Some st' => Ret (st', tt)
+            | None => throw Err end.                
+
+Definition err_write {E: Type -> Type} 
+  `{ErrState -< E} {S} (ms: option S) :
+  stateT S (itree E) unit :=
+  fun st => match ms with
+            | Some st' => Ret (st', tt)
+            | None => throw Err end.                
+
+Definition err_opt {E: Type -> Type} 
+  `{ErrState -< E} : option ~> itree E :=
+  fun _ t => match t with
+             | Some v => Ret v
+             | None => throw Err end.                
+
+Definition err_st_opt {E: Type -> Type} 
+  `{ErrState -< E} {S} : option ~> stateT S (itree E) :=
+  fun _ t st => match t with
+                | Some v => Ret (st, v)
+                | None => throw Err end.                
+
+End Errors.
+
+(*********************************************************************)
+
+(*
+Inductive instr_r :=
+| Cassgn   : lval -> assgn_tag -> stype -> pexpr -> instr_r
+| Copn     : lvals -> assgn_tag -> sopn -> pexprs -> instr_r
+| Csyscall : lvals -> syscall_t -> pexprs -> instr_r 
+| Cif      : pexpr -> seq instr -> seq instr  -> instr_r
+| Cfor     : var_i -> range -> seq instr -> instr_r
+| Cwhile   : align -> seq instr -> pexpr -> seq instr -> instr_r
+| Ccall    : lvals -> funname -> pexprs -> instr_r
+*)
+
+Section Lang.
+Context `{asmop:asmOp}.
+
+(** Events *)
+
+(* neutral reader events; here args and dests are meant to be symbolic
+locations associated to the function (concretely, stackframe
+locations) *)
+Variant FunE : Type -> Type :=
+  | FunCode (fn : funname) : FunE cmd
+  | FunArgs (fn: funname) : FunE lvals
+  | FunDests (fn: funname) : FunE lvals.                               
+
+(* neutral state events *)
+Variant StE : Type -> Type :=
+  | EvalCond (e: pexpr) : StE bool 
+  | EvalBound (e: pexpr) : StE Z
+  | WriteVar (x: var_i) (z: Z) : StE unit                             
+(* evaluates the expressions es and copy the values to la (local
+addresses in the stack frame) *)
+  | InitState (es: pexprs) (la: lvals) : StE unit
+(* copy the results in ld (local addesses in the stack frame) to gd
+(global ones) *)  
+  | SetDests (ld gd: lvals) : StE unit.  
+
+Variant InstrE : Type -> Type :=
+  | AssgnE : lval -> assgn_tag -> stype -> pexpr -> InstrE unit
+  | OpnE : lvals -> assgn_tag -> sopn -> pexprs -> InstrE unit
+  | SyscallE : lvals -> syscall_t -> pexprs -> InstrE unit. 
+  
+(* neutral mutual recursion events *)
+Variant CState : Type -> Type :=
+ | LCode (c: cmd) : CState unit
+ | FCall (xs: lvals) (f: funname) (es: pexprs) : CState unit.
+
+(** Auxiliary, for recursion on list (seq) *)
+
+Fixpoint cmd_map {E} (R: instr -> itree E unit)
+  (c: cmd) : itree E unit := 
+  match c with 
+  | nil => Ret tt 
+  | i :: c => R i ;; cmd_map R c
+  end.
+
+Fixpoint cmd_map_r {E} (R: instr_r -> itree E unit)
+  (c: cmd) : itree E unit := 
+  match c with 
+  | nil => Ret tt 
+  | (MkI _ i) :: c => R i ;; cmd_map_r R c
+  end.
+
+
+Section With_MREC.
+Context (Eff : Type -> Type)
+        (HasFunE : FunE -< Eff)
+        (HasStE : StE -< Eff)
+        (HasInstrE : InstrE -< Eff).   
+
+Definition denote_fcall (xs: lvals) (fn: funname) (es: pexprs) :
+  itree (CState +' Eff) unit :=
+  la <- trigger (FunArgs fn) ;;
+  trigger (InitState es la) ;; 
+  c <- trigger (FunCode fn) ;;   
+  trigger_inl1 (LCode c) ;; 
+  ld <- trigger (FunDests fn) ;; 
+  trigger (SetDests ld xs).
+
+Fixpoint denote_instr (i : instr_r) : itree (CState +' Eff) unit := 
+  let R := cmd_map_r denote_instr in
+  match i with
+  | Cassgn x tg ty e => trigger (AssgnE x tg ty e)
+  | Copn xs tg o es => trigger (OpnE xs tg o es)
+  | Csyscall xs o es => trigger (SyscallE xs o es)                          
+                                
+  | Cif e c1 c2 =>
+      b <- trigger (EvalCond e) ;;
+      if b then R c1 else R c2 
+
+  | Cfor i rng c =>
+      match rng with
+      | (d, e1, e2) =>
+          ITree.iter (fun _ =>
+            ITree.bind (trigger (EvalBound e1))
+            (fun lb => ITree.bind (trigger (EvalBound e2))
+            (fun ub =>                     
+            match (wrange d lb ub) with
+            | nil => ret (inr tt)
+            | (w :: ws) => trigger (WriteVar i w) ;; R c ;; ret (inl tt)
+            end))) tt
+      end
+        
+  | Cwhile a c1 e c2 => 
+      ITree.iter (fun _ =>
+           R c1 ;;          
+           b <- trigger (EvalCond e) ;;
+           if b then (R c2) ;; ret (inl tt) 
+           else ret (inr tt)) tt 
+  
+  | Ccall xs fn es => trigger_inl1 (FCall xs fn es)      
+  end.
+
+Definition denote_cstate : CState ~> itree (CState +' Eff) :=           
+  fun _ fs => match fs with
+              | LCode c => cmd_map_r denote_instr c
+              | FCall xs fn es => denote_fcall xs fn es       
+              end.      
+
+(* denotational interpreter *)
+Definition denote_cmd (c: cmd) : itree Eff unit :=
+  mrec denote_cstate (LCode c).
+
+(* for single instructions *)
+Definition denote_cmd1 (i: instr) : itree Eff unit :=
+  denote_cmd (i :: nil).
+
+End With_MREC.
+
+End Lang.
 
 
